theories/examples/iterated_ping_pong/proof.v
@@ -1,0 +1,1393 @@
+From iris.base_logic.lib Require Import invariants.
+From iris.algebra Require Import auth excl cmra gmap gset auth.
+From aneris.aneris_lang Require Import lifting tactics proofmode notation resources network state_interp.
+From aneris.aneris_lang.program_logic Require Import aneris_weakestpre
+     aneris_adequacy.
+From iris_string_ident Require Import ltac2_string_ident.
+From aneris.examples.iterated_ping_pong Require Export code.
+From RecordUpdate Require Import RecordSet.
+
+Import Network.
+Import String.
+Import RecordSetNotations.
+
+  Program Instance AndMon : Monoid and :=
+    {| monoid_unit := True |}.
+
+(* Network helpers *)
+Section network.
+
+  (* The network topology consists of a server and multiple clients.
+     All addresses are statically known. *)
+  Class NetworkTopo := mkTopo {
+    n_server : socket_address;
+    n_clients : gset socket_address;
+    n_all := n_clients ∪ {[ n_server ]};
+    addrs_disj : n_clients ## {[ n_server ]}
+  }.
+
+  Context `{!NetworkTopo}.
+
+  (* A ping message goes from the server to some client. *)
+  Definition mkPing (dest : socket_address) :=
+    {| m_sender := n_server;
+       m_destination := dest;
+       m_protocol := IPPROTO_UDP ;
+       m_body := "PING" |}.
+
+  (* A pong message goes from some client to the server. *)
+  Definition mkPong (sender : socket_address) :=
+    {| m_sender := sender;
+       m_destination := n_server;
+       m_protocol := IPPROTO_UDP ;
+       m_body := "PONG" |}.
+
+End network.
+
+(* Model definitions *)
+Section model.
+
+  Context `{!NetworkTopo}.
+
+  Definition msg_trace := list message.
+
+  Definition trace_to_gset := list_to_set (C := message_soup).
+
+  Definition app_msg (msgs : msg_trace) (msg : message) := msgs ++ [msg].
+
+  Notation "msgs ++_m m" := (app_msg msgs m) (at level 90, left associativity).
+
+  (* The transition relation of the STS *)
+  Inductive next : msg_trace -> msg_trace -> Prop :=
+  | next_ping msgs dest :
+      (* if we haven't already pinged the client *)
+      not (In (mkPing dest) msgs) ->
+      (* and the client address is valid *)
+      dest ∈ n_clients ->
+      (* then we can ping *)
+      next msgs (msgs ++_m (mkPing dest))
+  | next_pong msgs sender :
+      (* if we have already pinged the client that's responding *)
+      (In (mkPing sender) msgs) ->
+      (* and the client hasn't already responded *)
+      not (In (mkPong sender) msgs) ->
+      (* then the client can send a pong back *)
+      next msgs (msgs ++_m (mkPong sender)).
+
+  (* TODO: add tests for transition relation *)
+
+  Program Definition ping_pong_model : Model := {|
+    model_state := msg_trace;
+    model_rel := next
+  |}.
+  Next Obligation.
+  Admitted.
+  Next Obligation.
+  Admitted.
+End model.
+
+Notation "msgs ++_m m" := (app_msg msgs m) (at level 90, left associativity).
+
+Section ghost.
+  Record HandleSt := mkHandleSt {
+    handle : socket_handle;
+    skt : socket;
+    recv : message_soup;
+    sent : message_soup;
+  }.
+
+  Canonical Structure HandleStO := leibnizO HandleSt.
+
+  Definition handle_map := gmap socket_address HandleSt.
+
+  (* TODO: rename to something shorter *)
+  (* TODO: use big_opM *)
+  Definition handles_big_union `{EqDecision T} `{Countable T}
+             (m : handle_map) (f : socket_address -> HandleSt -> gset T) : gset T :=
+    map_fold (fun a st acc => acc ∪ (f a st)) ∅ m.
+
+  Notation "'[∪' 'map]' a ↦ st ∈ m , e" :=
+    (handles_big_union m (fun a st => e)) (at level 200, m at level 10, a, st at level 1).
+
+  Lemma handles_big_union_insert_new `{EqDecision T} `{Countable T}
+        (m : handle_map) (f : socket_address -> HandleSt -> gset T)
+        (k : socket_address) (k_st : HandleSt) :
+    m !! k = None ->
+    ([∪ map] a ↦ st ∈ <[ k := k_st ]> m, f a st) =
+    ([∪ map] a ↦ st ∈ m, f a st ) ∪ (f k k_st).
+  Proof.
+    intros Hnotin.
+    rewrite /handles_big_union.
+    rewrite map_fold_insert_L; [done | | done].
+    intros a1 a2 st1 st2 S Hne Ha1 Ha2.
+    set_solver.
+  Qed.
+
+  Lemma handles_big_union_insert_delete `{!EqDecision T} `{!Countable T}
+        (m : handle_map) (f : socket_address -> HandleSt -> gset T)
+        (k : socket_address) (k_st : HandleSt) :
+    ([∪ map] a ↦ st ∈ <[ k := k_st ]> m, f a st) =
+    (f k k_st) ∪ ([∪ map] a ↦ st ∈ delete k m, f a st).
+  Proof.
+    rewrite /handles_big_union.
+    rewrite -insert_delete map_fold_insert_L.
+    - set_solver.
+    - intros ? ? ? ? ? ? ? ?. set_solver.
+    - apply lookup_delete.
+  Qed.
+
+  Lemma elem_of_handles_big_union `{!EqDecision T} `{!Countable T}
+        (m : handle_map) (f : socket_address -> HandleSt -> gset T) (x : T) :
+        (x ∈ [∪ map] a ↦ st ∈ m, f a st) <-> (exists a st, m !! a = Some st /\ x ∈ f a st).
+  Proof.
+    induction m using map_ind; split.
+    - rewrite /handles_big_union.
+      rewrite map_fold_empty.
+      set_solver.
+    - intros [a [st [Hsome _]]].
+      rewrite lookup_empty in Hsome.
+      discriminate.
+    - rewrite /handles_big_union.
+      rewrite map_fold_insert_L; [| set_solver | done].
+      rewrite elem_of_union.
+      intros [Hl | Hr].
+      + rewrite /handles_big_union in IHm.
+        apply IHm in Hl as [a [st [Hsome Hin]]].
+        exists a, st.
+        rewrite lookup_insert_ne; [auto |].
+        intros ->.
+        rewrite H in Hsome.
+        discriminate.
+      + exists i, x0.
+        rewrite lookup_insert; auto.
+    - intros [a [st [Hsome Hf]]].
+      rewrite handles_big_union_insert_delete.
+      destruct (decide (a = i)) as [-> | ].
+      + rewrite lookup_insert in Hsome.
+        inversion Hsome; subst.
+        set_solver.
+      + rewrite lookup_insert_ne in Hsome; [ | auto].
+        rewrite delete_notin; [ | auto].
+        rewrite elem_of_union; right.
+        apply IHm; eauto.
+  Qed.
+
+  Definition freeUR : ucmra :=
+    authUR (gset_disjUR socket_address).
+
+  Definition handlesUR : ucmra :=
+    authUR (gmapUR socket_address (exclR HandleStO)).
+
+  (* TODO: find out why inlining this makes typeclass search fail *)
+  Definition handles_to_excl (m : handle_map) :
+    gmapUR socket_address (exclR HandleStO) :=
+    fmap Excl m.
+
+  Lemma handles_to_excl_invert (m : handle_map)
+        (a : socket_address) (st : HandleSt) :
+    handles_to_excl m !! a = Some (Excl st) -> m !! a = Some (st).
+  Proof.
+    rewrite lookup_fmap.
+    destruct (m !! a) as [st' | ] eqn:Heq; rewrite Heq;
+      simpl; intros H; [by inversion H | discriminate].
+  Qed.
+
+  (* The messages in the trace match the local view of what's been sent *)
+  Definition sent_consistent (mtrace : msg_trace) (handles : handle_map) : Prop :=
+    trace_to_gset mtrace = [∪ map] a ↦ st ∈ handles, st.(sent).
+
+  (* The local view of what's been received is a subset of the messages
+     in the trace. This is because not every sent message has been received. *)
+  Definition recv_consistent (mtrace : msg_trace) (handles : handle_map) : Prop :=
+   ([∪ map] a ↦ st ∈ handles, st.(recv)) ⊆ trace_to_gset mtrace.
+
+  Definition pingTokR : cmra := exclR natO.
+
+  (* Ghost and invariant names used throughout the example *)
+  Class GhostInvNames `{!NetworkTopo} := mkGhostnames {
+    (* Name for the state that tracks free handles *)
+    γ_free : gname;
+    (* Name for the state that tracks active handles *)
+    γ_handles : gname;
+    (* Generate ghost names for client tokens.
+       It's up to the user to define the domain ... *)
+    gen_tok_name : socket_address -> option gname;
+    (* ... but it should be at least all client addresses *)
+    gen_tok_name_defined :
+      forall (a : socket_address), a ∈ n_clients -> is_Some (gen_tok_name a);
+    (* The name of the global protocol invariant *)
+    inv_ns : namespace
+  }.
+
+
+
+End ghost.
+
+Section inv.
+  Context `{!NetworkTopo}.
+  Context `{!GhostInvNames}.
+  Context `{distG : !anerisG ping_pong_model Σ}.
+  Context `{!inG Σ freeUR}.
+  Context `{!inG Σ handlesUR}.
+  Context `{!inG Σ pingTokR}.
+
+  Definition handle_st_to_mapsto (a : socket_address) (st : HandleSt) : iProp Σ :=
+    st.(handle) ↪[ip_of_address a] st.(skt) ∗ a ⤳ (st.(recv), st.(sent)).
+
+  Definition free_addrs (F : gset socket_address) : iProp Σ :=
+    [∗ set] a ∈ F, free_ports (ip_of_address a) {[port_of_address a]}.
+
+  Definition mapsto_handles (hs : handle_map) : iProp Σ :=
+    ([∗ map] a ↦ st ∈ hs, handle_st_to_mapsto a st).
+
+  Definition auth_handles (hs : handle_map) : iProp Σ :=
+    own γ_handles (● (handles_to_excl hs)).
+
+  (*
+   * Given a resource a ↪ (handle, skt, recv, sent):
+   *   1) the socket address must be `a`
+   *   2) all messages in `recv` must have `a` as destination
+   *   3) all mesages in `sent` must have `a` as source
+   *)
+  (* TODO: make this a pure proposition *)
+  Definition handle_addr_match (a : socket_address) (st : HandleSt) : iProp Σ :=
+    (⌜st.(skt).(saddress) = Some a⌝ ∗
+     ([∗ set] m ∈ st.(recv), ⌜m_destination m = a⌝) ∗
+     ([∗ set] m ∈ st.(sent), ⌜m_sender m = a⌝))%I.
+
+  Definition handle_addrs_match (hs : handle_map) : iProp Σ :=
+    [∗ map] a ↦ st ∈ hs, handle_addr_match a st.
+
+  Definition generic_inv (mdl_st : ping_pong_model) : iProp Σ :=
+    ∃ (P F : gset socket_address) (handles : handle_map),
+      (* We can split all addresses A into participating addresses P and
+         free addresses F *)
+      (* Both sets are disjoint *)
+      ⌜P ## F⌝ ∗
+      (* Ghost state that tracks free addresses, so we can pull information
+         out of the invariant *)
+      own γ_free (● (GSet F)) ∗
+      (* The ghost state that tracks participating addresses tracks the
+         right addresses *)
+      ⌜dom _ handles = P⌝ ∗
+      (* The authoritative part that tracks participating addresses *)
+      auth_handles handles ∗
+      (* The handle states are consistent with their key (address) *)
+      handle_addrs_match handles ∗
+      (* We have mapsto for every participating address *)
+      mapsto_handles handles ∗
+      (* The current state of the model *)
+      frag_st mdl_st ∗
+      (* Our tracking of sends is consistent with the model *)
+      ⌜sent_consistent mdl_st handles⌝ ∗
+      (* Our tracking of receives is consistent with the model *)
+      ⌜recv_consistent mdl_st handles⌝.
+
+  (* Generates optional ping tokens *)
+  Definition ping_tok (a : socket_address) : iProp Σ :=
+    match (gen_tok_name a) with
+    | Some γ => own γ (Excl 0)
+    | None => True
+    end.
+
+  Definition ping_pong_inv : iProp Σ :=
+    ∃ (mdl_st : ping_pong_model),
+      generic_inv mdl_st ∗
+      (* If we have a ping token we can know that the corresponding ping
+         message has been recorded in the model trace *)
+      ([∗ set] a ∈ n_clients, ((ping_tok a) ∨ ⌜In (mkPing a) mdl_st⌝)%I).
+
+  (* User-level resource indicating that the given address is free *)
+  Definition ufree (a : socket_address) : iProp Σ :=
+    own γ_free (◯ GSet {[ a ]}).
+
+  (* User resource for tracking an allocated socket handle *)
+  Definition uhandle (a : socket_address) (st : HandleSt) : iProp Σ :=
+    own γ_handles (◯ {[ a := Excl st ]}).
+
+  Notation "a '↪h' '(' h ',' s ',' R ',' S ')'" :=
+    (uhandle a (mkHandleSt h s R S)) (at level 90).
+
+  (* We now prove some helper lemmas that help us work with the invariant *)
+
+  (* If we have the user free resource we can recover
+     the socket free resource *)
+  Lemma ufree_free (a : socket_address) (F : gset socket_address) :
+    ufree a -∗
+    own γ_free (● (GSet F)) -∗
+    (ufree a ∗
+     ⌜a ∈ F⌝ ∗
+     own γ_free (● (GSet F))).
+  Proof.
+    iIntros "Hfrag Hauth".
+    iDestruct (own_valid_2 with "Hauth Hfrag") as
+        %[Helem%gset_disj_included
+               %elem_of_subseteq_singleton _] %auth_both_valid_discrete.
+    iFrame. done.
+  Qed.
+
+  Lemma uhandle_handles_some (a : socket_address)
+                             (h : socket_handle)
+                             (skt : socket)
+                             (R S : gset message)
+                             (handles : handle_map) :
+    a ↪h (h, skt, R, S) -∗
+    auth_handles handles -∗
+    ⌜handles !! a = Some (mkHandleSt h skt R S)⌝.
+  Proof.
+    iIntros "Hfrag Hauth".
+    iDestruct (own_valid_2 with "Hauth Hfrag") as
+        %[Hincl Hv]%auth_both_valid_discrete.
+    apply (singleton_included_exclusive_l _ _ _ _ Hv) in Hincl.
+    apply leibniz_equiv in Hincl.
+    apply handles_to_excl_invert in Hincl.
+    by iPureIntro.
+  Qed.
+
+  (* If we have the user socket handle we can recover
+     the socket mapsto resource *)
+  Lemma uhandle_handle (a : socket_address)
+                       (h : socket_handle)
+                       (s : socket)
+                       (R S : gset message)
+                       (handles : handle_map) :
+    a ↪h (h, s, R, S) -∗
+    auth_handles handles -∗
+    mapsto_handles handles -∗
+    (a ↪h (h, s, R, S) ∗
+     auth_handles handles ∗
+     handle_st_to_mapsto a (mkHandleSt h s R S) ∗
+     mapsto_handles (delete a handles) ∗
+     ⌜handles !! a = Some (mkHandleSt h s R S)⌝).
+  Proof.
+    iIntros "Hfrag Hauth Hmapsto".
+    iDestruct (uhandle_handles_some with "Hfrag Hauth") as %Hincl.
+    iPoseProof (big_opM_delete _ _ _) as "Hrw"; [eassumption|].
+    iDestruct ("Hrw" with "Hmapsto") as "[? ?]"; iFrame.
+    by iPureIntro.
+  Qed.
+
+  (* We can simultaneously allocate a uhandle and
+     the corresponding socket mapsto *)
+  Lemma uhandle_alloc (a : socket_address)
+                      (sh : socket_handle)
+                      (s : socket)
+                      (handles : handle_map)
+                      (R S : message_soup) :
+    ⌜a ∉ dom (gset socket_address) handles⌝ -∗
+    auth_handles handles -∗
+    mapsto_handles handles -∗
+    sh ↪[ ip_of_address a] s -∗ a ⤳ (R, S) ==∗
+    let handles' := <[ a := mkHandleSt sh s R S ]> handles in
+      a ↪h (sh, s, R, S) ∗
+      auth_handles handles' ∗
+      mapsto_handles handles'.
+  Proof.
+    iIntros "%Hnotin Hauth Hsh Hmapsto Hleadsto".
+    iMod (own_update _ _
+           (● (handles_to_excl (<[ a := mkHandleSt sh s R S ]> handles )) ⋅
+            ◯ {[ a := Excl (mkHandleSt sh s R S)]}) with "Hauth")
+      as "Halloc".
+    { apply auth_update_alloc.
+      rewrite /handles_to_excl.
+      rewrite fmap_insert.
+      (* Had to supply the RA manually for some reason *)
+      apply (alloc_singleton_local_update (A := exclR HandleStO));
+        [ | by constructor ].
+      rewrite lookup_fmap.
+      assert (Hnone: handles !! a = None).
+      { apply not_elem_of_dom; assumption. }
+      by rewrite Hnone.
+    }
+    iDestruct (own_op with "Halloc") as "[Hauth Hfrag]".
+    iModIntro; iFrame.
+    iApply (big_sepM_insert_2 with "[Hmapsto Hleadsto] Hsh").
+    iFrame. (* TODO: why can't we frame this directly in the line above. *)
+   Qed.
+
+  (* We can delete from the authoritative ufree set *)
+  Lemma ufree_delete (F : gset socket_address) (a : socket_address ) :
+    own γ_free (● GSet F) -∗
+    ufree a ==∗
+    own γ_free (● GSet (F ∖ {[ a ]})).
+  Proof.
+    iIntros "Hauth Hfrag".
+    iMod (own_update_2 with "Hauth Hfrag");
+      last by iFrame.
+    apply auth_update_dealloc.
+    apply gset_disj_dealloc_local_update.
+  Qed.
+
+  Lemma delete_insert_eq (m : handle_map) (i : socket_address) (x : HandleSt) :
+    m !! i = Some x ->
+    <[ i := x ]> (delete i m) = m.
+  Proof.
+    intros Hsome.
+    rewrite insert_delete.
+    apply insert_id; assumption.
+  Qed.
+
+  Lemma mapsto_reconstitute (sh : socket_handle)
+                            (a : socket_address)
+                            (skt : socket)
+                            (handles : handle_map)
+                            (R S : gset message) :
+    ⌜handles !! a = Some (mkHandleSt sh skt R S)⌝ -∗
+    sh ↪[ ip_of_address a] skt -∗ a ⤳ (R, S) -∗
+    mapsto_handles (delete a handles) -∗
+    mapsto_handles handles.
+  Proof.
+    iIntros "%Hsome Hsh Hmapsto Hleadsto".
+    iDestruct (big_sepM_insert handle_st_to_mapsto
+                               (delete a handles)
+                               a
+                               (mkHandleSt sh skt R S)
+                 with "[Hsh Hmapsto Hleadsto]") as "Hmapsto'".
+    - apply lookup_delete_None; auto.
+    - iFrame.
+    - rewrite delete_insert_eq; [iFrame | assumption].
+  Qed.
+
+  Lemma mapsto_reconstitute_new (sh : socket_handle)
+                                (a : socket_address)
+                                (skt : socket)
+                                (handles : handle_map)
+                                (R S : gset message) :
+    sh ↪[ ip_of_address a] skt -∗ a ⤳ (R, S) -∗
+    mapsto_handles (delete a handles) -∗
+    mapsto_handles (<[ a := mkHandleSt sh skt R S ]> handles).
+  Proof.
+    rewrite /mapsto_handles.
+    iIntros "Hsh Hmapsto Hleadsto".
+    remember {| handle := sh; skt := skt; recv := R; sent := S |} as st'.
+    assert (<[a:=st']> handles = <[a := st' ]> (delete a handles)) as ->.
+    { rewrite insert_delete; done. }
+    rewrite big_sepM_insert; [ | apply lookup_delete].
+    rewrite /handle_st_to_mapsto; subst; simpl.
+    iFrame.
+  Qed.
+
+  Lemma handles_to_excl_insert (handles : handle_map)
+                               (a : socket_address)
+                               (st : HandleSt) :
+    handles_to_excl (<[a:=st]> handles) = <[a := Excl st]> (handles_to_excl handles).
+  Proof.
+    rewrite /handles_to_excl.
+    by rewrite fmap_insert.
+  Qed.
+
+  Lemma uhandle_update (a : socket_address)
+                       (handles : handle_map)
+                       (st st' : HandleSt) :
+    ⌜handles !! a = Some st⌝ -∗
+    auth_handles handles -∗
+    uhandle a st ==∗
+    auth_handles (<[ a := st' ]> handles) ∗
+    uhandle a st'.
+  Proof.
+    iIntros "%Hsome Hauth Hfrag".
+    iApply own_op.
+    iApply (own_update_2 with "Hauth Hfrag").
+    apply auth_update.
+    rewrite handles_to_excl_insert.
+    rewrite -[({[_ := Excl st']})](insert_singleton _ (Excl st)).
+    apply (insert_local_update _ _ _ (Excl st) (Excl st)).
+    - rewrite /handles_to_excl.
+      by rewrite lookup_fmap Hsome.
+    - by rewrite lookup_singleton.
+    - apply exclusive_local_update; done.
+  Qed.
+
+  Lemma handle_addrs_match_insert (handles : handle_map)
+                                  (a : socket_address)
+                                  (st st' : HandleSt) :
+    handle_addrs_match handles -∗
+    ⌜handles !! a = Some st⌝ -∗
+    handle_addr_match a st' -∗
+    handle_addrs_match (<[a := st']> handles).
+  Proof.
+    iIntros "Hmatch %Hsome Hmatch_st'".
+    rewrite /handle_addrs_match.
+    assert (handles = <[a := st]> handles) as ->.
+    { rewrite insert_id; eauto. }
+    do 2 rewrite big_sepM_insert_delete.
+    rewrite delete_insert_delete.
+    iDestruct "Hmatch" as "[_ ?]".
+    iFrame.
+  Qed.
+
+  Lemma extract_ping_tok (a : socket_address)
+                         (mdl : msg_trace) :
+    ⌜a ∈ n_clients⌝ -∗
+    ping_tok a -∗
+    ([∗ set] a ∈ n_clients, ping_tok a ∨ ⌜In (mkPing a) mdl⌝) -∗
+    (([∗ set] a ∈ n_clients, ping_tok a ∨ ⌜In (mkPing a) mdl⌝) ∗
+     ⌜In (mkPing a) mdl⌝).
+  Proof.
+    iIntros "%Hin Htok Hall".
+    iDestruct (big_sepS_elem_of_acc _ _ a with "Hall") as
+        "[[Htok' | Hin]  Himpl]"; try done.
+    - (* duplicated token: contradiction *)
+      iExFalso.
+      rewrite /ping_tok.
+      destruct (gen_tok_name_defined a Hin) as [nm ->].
+      by iDestruct (own_valid_2 with "Htok Htok'") as "%Hvalid".
+    - (* ping in trace *)
+      iFrame.
+      iApply "Himpl"; eauto.
+  Qed.
+
+  Lemma sent_consistent_after_receive (handles : handle_map)
+                                      (a : socket_address)
+                                      (st st' : HandleSt)
+                                      (mdl : msg_trace) :
+    sent_consistent mdl handles ->
+    handles !! a = Some st ->
+    st.(sent) = st'.(sent) ->
+    sent_consistent mdl (<[a := st']> handles).
+  Proof.
+    rewrite /sent_consistent.
+    intros Hcons Hsome Heq.
+    rewrite handles_big_union_insert_delete.
+    rewrite -[handles](insert_id _ a st) in Hcons; [ | assumption].
+    rewrite Hcons handles_big_union_insert_delete Heq.
+    reflexivity.
+  Qed.
+
+  Lemma sent_consistent_after_send (handles : handle_map)
+                                   (a : socket_address)
+                                   (st st' : HandleSt)
+                                   (mdl : msg_trace)
+                                   (m : message) :
+    sent_consistent mdl handles ->
+    handles !! a = Some st ->
+    st'.(sent) = st.(sent) ∪ {[ m ]} ->
+    sent_consistent (mdl ++_m m) (<[a := st']> handles).
+  Proof.
+    rewrite /sent_consistent.
+    intros Hcons Hsome Heq.
+    rewrite handles_big_union_insert_delete.
+    rewrite -[handles](insert_id _ a st) in Hcons; [ | assumption].
+    rewrite /trace_to_gset /app_msg.
+    rewrite list_to_set_app_L Heq; simpl.
+    rewrite union_empty_r_L.
+    assert (list_to_set mdl = sent st ∪ handles_big_union (delete a handles) (λ (_ : socket_address) (st : HandleSt), sent st)) as ->; [ | set_solver].
+    rewrite /trace_to_gset in Hcons.
+    rewrite handles_big_union_insert_delete in Hcons.
+    set_solver.
+  Qed.
+
+  Lemma in_subseteq (m : message) (mdl : msg_trace) :
+    In m mdl -> {[m]} ⊆ trace_to_gset mdl.
+  Proof.
+    intros Hin.
+    rewrite -elem_of_subseteq_singleton
+             elem_of_list_to_set
+             elem_of_list_In; done.
+  Qed.
+
+  Lemma recv_consistent_after_receive (handles : handle_map)
+                                      (a : socket_address)
+                                      (st st' : HandleSt)
+                                      (mdl : msg_trace)
+                                      (m : message) :
+    recv_consistent mdl  handles ->
+    handles !! a = Some st ->
+    st.(recv) ∪ {[m]} = st'.(recv) ->
+    In m mdl ->
+    recv_consistent mdl (<[a := st']> handles).
+  Proof.
+    rewrite /recv_consistent.
+    intros Hcons Hsome Hsub Hin.
+    rewrite handles_big_union_insert_delete.
+    rewrite -[handles](insert_id _ a st) in Hcons; [ | assumption].
+    rewrite handles_big_union_insert_delete in Hcons.
+    apply union_least; [ | set_solver].
+    rewrite -Hsub.
+    apply union_least; [set_solver |].
+    apply in_subseteq; done.
+  Qed.
+
+  Lemma recv_consistent_after_send (handles : handle_map)
+                                   (a : socket_address)
+                                   (st st' : HandleSt)
+                                   (mdl : msg_trace)
+                                   (m : message) :
+    recv_consistent mdl handles ->
+    handles !! a = Some st ->
+    st'.(recv) = st.(recv) ->
+    recv_consistent (mdl ++_m m) (<[a := st']> handles).
+  Proof.
+    rewrite /recv_consistent.
+    intros Hcons Hsome Heq.
+    rewrite /trace_to_gset /app_msg list_to_set_app.
+    rewrite handles_big_union_insert_delete.
+    rewrite -(delete_insert_eq handles a st) in Hcons; [ | assumption].
+    rewrite handles_big_union_insert_delete in Hcons.
+    rewrite delete_idemp in Hcons.
+    apply union_subseteq in Hcons as [HL HR].
+    rewrite /trace_to_gset in HL.
+    apply union_subseteq; set_solver.
+  Qed.
+
+  Lemma recv_consistent_elem (msgs : msg_trace)
+                             (handles : handle_map)
+                             (a : socket_address)
+                             (st : HandleSt)
+                             (m : message) :
+    recv_consistent msgs handles ->
+    handles !! a = Some st ->
+    m ∈ st.(recv) ->
+    m ∈ msgs.
+  Proof.
+    rewrite /recv_consistent /trace_to_gset.
+    intros Hcons Hsome Hin.
+    rewrite <- elem_of_list_to_set.
+    assert (H': m ∈ handles_big_union handles (λ (_ : socket_address) (st : HandleSt), recv st)); [ | set_solver].
+    rewrite elem_of_handles_big_union; eauto.
+  Qed.
+
+  Lemma sent_consistent_elem (msgs : msg_trace)
+                             (handles : handle_map)
+                             (a : socket_address)
+                             (st : HandleSt)
+                             (m : message) :
+    ⌜sent_consistent msgs handles⌝ -∗
+    ⌜handles !! a = Some st⌝ -∗
+    ⌜m ∈ msgs⌝ -∗
+    ⌜m_sender m = a⌝ -∗
+    handle_addrs_match handles -∗
+    ⌜m ∈ st.(sent)⌝.
+  Proof.
+    rewrite /handle_addrs_match /sent_consistent.
+    iIntros "%Hcons %Hsome %Hin %Hsender Hmatch".
+    rewrite /trace_to_gset in Hcons.
+    rewrite <- elem_of_list_to_set in Hin.
+    assert (Hin': m ∈ handles_big_union handles
+                    (λ (_ : socket_address) (st : HandleSt), sent st)).
+    { set_solver. }
+    apply elem_of_handles_big_union in Hin' as [a' [st' [Hsome' Hin']]].
+    iDestruct ((big_sepM_lookup handle_addr_match handles a') with "Hmatch")
+      as "(%H1 & _ & H3)"; [eauto |].
+    iDestruct (big_sepS_elem_of _ _ _ Hin' with "H3") as "%Heq"; subst.
+    rewrite Hsome in Hsome'.
+    inversion Hsome'; auto.
+  Qed.
+
+  From aneris Require Import lib.util.
+
+  From aneris Require Import program_logic.adequacy.
+  (* Lemma socket_state_same_one σ κs k *)
+  (*       (δ: aux_state (@aneris_AS ping_pong_model)) a hst: *)
+  (*      state_interp σ δ κs k -∗ *)
+  (*       handle hst ↪[ ip_of_address a] skt hst -∗ a ⤳ (recv hst, sent hst) -∗ *)
+  (*       ⌜ match σ with *)
+  (*           mkState _ c_skts c_in_use _ => *)
+  (*           ∃ c_skt_map : sockets, *)
+  (*                          c_skts !! ip_of_address a = Some c_skt_map *)
+  (*                          ∧ (∃ (c_skt : socket) (R S : gset message), *)
+  (*                               c_skt_map !! handle hst = Some (c_skt, R, S) *)
+  (*                               ∧ c_skt = skt hst ∧ R = recv hst ∧ S = sent hst) *)
+  (* end⌝. *)
+  (* Proof. *)
+  (*   iIntros "Hsi Hhan". *)
+  (*   unfold state_interp, anerisG_irisG. Search aneris_state_interp. *)
+  (*   iPoseProof (aneris_state_interp_socket_valid with "[$] [$]") as (hh) "%Hh". *)
+  (*   destruct Hh as [Hh Hh']. *)
+  (*   iPureIntro. destruct σ as [A B C D]. simpl in Hh. exists hh. *)
+  (*   split; first done. by do 3 eexists. *)
+  (* Qed. *)
+
+  (* Lemma socket_state_same σ κs k st (handles: handle_map):  *)
+  (*      state_interp σ κs k st -∗ *)
+  (*       ([∗ map] a↦hst ∈ handles,  handle hst ↪[ ip_of_address a ] (skt hst, recv hst, sent hst)) -∗ *)
+  (*       ⌜ match σ with *)
+  (*           mkState _ c_skts c_in_use _ => *)
+  (*             ([^ and map] a↦hst ∈ handles, *)
+  (*               exists c_skt_map : sockets, *)
+  (*                 c_skts !! (ip_of_address a) = Some c_skt_map /\ *)
+  (*                 exists (c_skt : socket) (R S : gset message), *)
+  (*                   c_skt_map !! hst.(handle) = Some (c_skt, R, S) /\ *)
+  (*                   c_skt = hst.(skt) /\ *)
+  (*                   R = hst.(recv) /\ *)
+  (*                   S = hst.(sent)) *)
+  (*         end⌝. *)
+  (* Proof. *)
+  (*   induction handles as [| a hst handles Hnotin IH] using map_ind; iIntros "Hst H"; destruct σ; *)
+  (*    first by iPureIntro;  rewrite big_opM_empty.  *)
+  (*   rewrite !big_opM_insert //. iDestruct "H" as "[H Hr]". *)
+  (*   iSplit. *)
+  (*   - by iPoseProof (socket_state_same_one with "Hst H") as "?". *)
+  (*   - by iApply (IH with "[$]"). *)
+  (* Qed.       *)
+
+End inv.
+
+Notation "a '↪h' '(' h ',' s ',' R ',' S ')'" :=
+  (uhandle a (mkHandleSt h s R S)) (at level 90).
+
+Section client.
+  Context `{!NetworkTopo}.
+  Context `{!GhostInvNames}.
+  Context `{!inG Σ freeUR}.
+  Context `{!inG Σ handlesUR}.
+  Context `{!inG Σ pingTokR}.
+  Context `{distG : !anerisG ping_pong_model Σ}.
+
+  Definition client_si (a : socket_address) : socket_interp Σ :=
+    (λ msg, (ping_tok a) ∗
+            ⌜msg = mkPing a⌝ ∗
+            (∃ ϕ, m_sender msg ⤇ ϕ ∗
+                 ∀ m, ⌜m = mkPong a⌝ -∗ ϕ m))%I.
+
+  Lemma client_spec (client_addr : socket_address)
+                    (ip : ip_address) :
+    ip = ip_of_address client_addr ->
+    client_addr ∈ n_clients ->
+    inv inv_ns ping_pong_inv -∗
+    fixed n_all -∗
+    ufree client_addr -∗
+    free_ports (ip_of_address client_addr) {[ port_of_address client_addr ]} -∗
+    client_addr ⤇ client_si client_addr -∗
+    client_addr ⤳ (∅, ∅) -∗
+    WP client #client_addr @[ip] {{ v, True }}.
+  Proof.
+    iIntros (-> Hin) "#Hinv #Hfixed Hufree Hfreeport #Hsi Hlt".
+    rewrite /client. wp_pures.
+    (* Allocate the socket *)
+    wp_bind (NewSocket _ _ _)%E.
+    wp_socket sh as "Hsh". wp_pures.
+    (* Static bind the socket, for which we need to open the invariant *)
+    wp_bind (SocketBind _ _).
+    iInv inv_ns as (mdl) "> (Hgen & Htoks)" "Hclose".
+    iDestruct "Hgen" as (P F handles) "(%Hdisj & Hfree_auth &
+              %Hdom & Hauth_handles & #Haddrs_match & Hmapsto & Hrest)".
+    assert (Hin_all: client_addr ∈ n_all) by set_solver.
+    iDestruct (ufree_free with "Hufree Hfree_auth") as
+        "(Hufree & %Helem & Hfree_auth)".
+    wp_socketbind_static.
+    (* Now close the invariant *)
+    iMod (ufree_delete with "Hfree_auth Hufree") as "Hfree_auth".
+    iMod (uhandle_alloc with "[] Hauth_handles Hmapsto Hsh Hlt") as
+        "(Huhandle & Hauth_handles' & Hmapsto')".
+    { iPureIntro; subst ; set_solver. }
+    iMod ("Hclose" with "[Htoks Hfree_auth Hrest Hauth_handles' Hmapsto']") as "_".
+    { iNext. iExists mdl.
+      iFrame.
+      iExists (P ∪ {[ client_addr ]}), (F ∖ {[ client_addr ]}), _.
+      iDestruct "Hrest" as "(Hfrag & %Hsent & %Hrecv)".
+      iFrame.
+      repeat iSplit; try iPureIntro.
+      - set_solver.
+      - set_solver.
+      - unfold handle_addrs_match.
+        iApply big_sepM_insert.
+        { apply not_elem_of_dom; set_solver. }
+        iFrame "#".
+        repeat iSplit; eauto.
+      - unfold sent_consistent.
+        rewrite handles_big_union_insert_new;
+          (try apply not_elem_of_dom); set_solver.
+      - unfold recv_consistent.
+        rewrite handles_big_union_insert_new;
+          (try apply not_elem_of_dom); set_solver.
+    }
+    iModIntro; wp_pures.
+    wp_bind (ReceiveFrom _).
+
+    clear mdl. (* It's ok to forget about the old state of the model *)
+    iInv inv_ns as (mdl) "> (Hgen & Htoks)".
+    iClear "Haddrs_match".
+    clear Hdisj Hdom Helem P F handles.
+    iDestruct "Hgen" as (P F handles) "(%Hdisj & Hfree_auth &
+            %Hdom & Hauth_handles & #Haddrs_match & Hmapsto & Hmdl & %Hscons & %Hrcons)".
+    iDestruct (uhandle_handle with "Huhandle Hauth_handles Hmapsto") as
+        "(Huhandle & Hauth_handles & Hmapsto & Hmapsto_rest & %Hsome)".
+
+    remember (udp_socket (Some client_addr) true) as skt eqn:Heq.
+    iAssert (⌜ handle_st_to_mapsto client_addr {| handle := sh; skt := skt; recv := ∅; sent := ∅ |} = (sh ↪[ ip_of_address client_addr] skt ∗ client_addr ⤳ (∅, ∅)) ⌝%I) as "->".
+    { iPureIntro; reflexivity. }
+
+    wp_apply (aneris_wp_receivefrom _ _ _ _ (udp_socket (Some _) true) with "[Hmapsto]") => //.
+    { iFrame "Hsi". iApply bi.later_sep_1; iNext. subst. iFrame. }
+
+    iIntros (msg) "(Hsh&Hmsg)".
+    iDestruct "Hmsg" as "[(#Hnotin & Hleadsto & Hsi_ok) | [%?]]";
+      last by set_solver.
+    remember (mkHandleSt sh skt {[mkPing client_addr]} ∅) as st'.
+    iMod (uhandle_update _ _ _ st' with
+              "[//] Hauth_handles Huhandle") as "[Hauth_handles Huhandle]".
+    unfold client_si.
+    iDestruct "Hsi_ok" as "(Hclienthist & Hclient & Htok & -> & Hsi_ok)".
+    iDestruct (extract_ping_tok with "[//] Htok Htoks") as "[Htoks %Hping]".
+    iModIntro. iSplitR "Huhandle Hsi_ok".
+    { iNext. iExists mdl; iFrame.
+    iExists P, F, (<[ client_addr := st' ]> handles). iFrame "∗#".
+    iSplit; [by iPureIntro |].
+    iSplit.
+    { iPureIntro. rewrite -Hdom dom_insert_L.
+      have Hindom: client_addr ∈ dom (gset socket_address) handles
+        by rewrite elem_of_dom Hsome; eauto.
+      set_solver. }
+    iSplitR.
+    { iApply handle_addrs_match_insert; eauto with iFrame.
+      repeat iSplit; rewrite Heqst'; eauto.
+      * by rewrite Heq.
+      * by rewrite big_sepS_singleton. }
+    iSplitL "Hleadsto Hmapsto_rest Hsh Hclienthist".
+    { rewrite /mapsto_handles  big_sepM_insert_delete.
+      rewrite /handle_st_to_mapsto Heqst'; simpl.
+      rewrite union_empty_r_L.
+      subst; iFrame. }
+    iSplit.
+    { iPureIntro.
+      eapply sent_consistent_after_receive; eauto.
+      rewrite Heqst'; reflexivity. }
+    iPureIntro.
+    eapply recv_consistent_after_receive; eauto.
+    rewrite Heqst'; set_solver. }
+    wp_apply wp_unSOME =>//; iIntros "_".
+    wp_pures.
+
+
+    clear mdl Hscons Hrcons Hping. (* It's ok to forget about the old state of the model *)
+    iClear "Haddrs_match".
+    clear Hdisj Hdom P F handles Hsome.
+
+    iApply (aneris_wp_atomic_take_step_model) =>//.
+    iInv inv_ns as (mdl) "> (Hgen & Htoks)" "Hclose"; iModIntro.
+    iDestruct "Hgen" as (P F handles) "(%Hdisj & Hfree_auth & %Hdom & Hauth_handles & #Haddrs_match & Hmapsto & Hfrag_mdl & %Hscons & %Hrcons)".
+    remember (mdl ++_m (mkPong client_addr)) as mdl'.
+    iExists mdl, mdl'.
+
+    destruct st' as [h skt' R S].
+    iDestruct (uhandle_handles_some with "Huhandle Hauth_handles") as "%Hsome".
+    pose proof (recv_consistent_elem _ _ _ _
+                   (mkPing client_addr) Hrcons Hsome) as Hin_mdl.
+    iAssert (⌜(mkPing client_addr) ∈ mdl⌝%I) as "%Hping_in".
+    { iPureIntro. set_solver. }
+    (* Show that (mkPong client_addr) ∉ mdl' *)
+    iAssert (⌜(mkPong client_addr) ∉ mdl⌝%I) as "%Hpong_notin".
+    { iIntros (contra).
+      iDestruct (sent_consistent_elem with "[] [] [] [] Haddrs_match")
+        as "%Hpong_in"; eauto with iFrame.
+      rewrite Heqst' in Hpong_in. set_solver. }
+
+    iFrame; iSplit.
+    { iPureIntro. rewrite Heqmdl'.
+      apply next_pong; rewrite <- elem_of_list_In; assumption. }
+
+    (* Pick out socket protocol and apply wp_send *)
+    iDestruct (uhandle_handle with "Huhandle Hauth_handles Hmapsto") as
+          "(Huhandle & Hauth_handles & [Hmapstoph Hmapstolog] & Hmapsto_rest & _)".
+    rewrite /handle_addrs_match.
+    injection Heqst'. intros **; subst.
+    iDestruct ((big_sepM_lookup _ _ client_addr
+                               {| handle := sh;
+                                  skt := udp_socket (Some client_addr) true;
+                                  recv := {[mkPing client_addr]} ;
+                                  sent := ∅ |}) with "Haddrs_match") as
+        "(%addr_ok & _ & _)"; [done|].
+    simpl in addr_ok; subst.
+    iDestruct "Hsi_ok" as (ϕ) "[Hsender Hres]".
+    simpl.
+    wp_apply (aneris_wp_send _ ϕ _ _ _ _ _
+                             (udp_socket (Some client_addr) true)
+                with "[Hmapstolog Hmapstoph Hsender Hres]"); eauto.
+    unfold handle_st_to_mapsto.
+    +  iFrame "∗#". iModIntro. by iApply "Hres".
+    + iIntros "[Hshph Hshlog] Hfrag".
+      simpl.
+      remember (mkHandleSt sh
+                           (udp_socket (Some client_addr) true)
+                           {[mkPing client_addr]}
+                           {[mkPong client_addr]}) as st' eqn:Heq.
+      iMod (uhandle_update _ _ _ st' with
+                "[//] Hauth_handles Huhandle") as "[Hauth_handles' Huhandle']".
+      assert ({| m_sender := client_addr; m_destination := n_server; m_protocol := IPPROTO_UDP; m_body := "PONG" |} = (mkPong client_addr)) as ->; [auto |].
+      iAssert ((mapsto_handles (<[ client_addr := st' ]> handles)))
+        with "[Hmapsto_rest Hshlog Hshph]" as "Hmapsto'".
+      { rewrite Heq.
+        assert ({[mkPong client_addr]} ∪ ∅ = {[mkPong client_addr]}) as ->.
+        { set_solver. }
+        iApply (mapsto_reconstitute_new with "[$] [$] [$]"). }
+      iMod ("Hclose" with "[-]") as "_"; last done.
+      iModIntro.
+      rewrite /ping_pong_inv /generic_inv.
+      iExists (mdl ++_m mkPong client_addr).
+      iSplitR "Htoks"; last first.
+      { iApply (big_sepS_impl with "Htoks").
+        iModIntro.
+        iIntros (x) "_ [Htok | %Hin']"; [iLeft; iFrame |].
+        iRight; iPureIntro.
+        apply in_or_app; auto. }
+      iExists  (dom (gset socket_address) handles),
+               F,
+               (<[client_addr:=st']> handles).
+      iFrame; iFrame "#".
+      iSplitL ""; [iPureIntro; assumption |].
+      iSplitL ""; [iPureIntro |].
+      { rewrite dom_insert_L.
+        rewrite subseteq_union_1_L; [reflexivity |].
+        rewrite -elem_of_subseteq_singleton elem_of_dom; eauto. }
+      iSplitL "Haddrs_match".
+      { rewrite /handle_addrs_match.
+        rewrite -insert_delete big_sepM_insert; [ | apply lookup_delete].
+        iSplitL "".
+        - rewrite /handle_addr_match Heq; simpl.
+          iSplitL; [done |].
+          do 2 (rewrite big_sepS_singleton); iPureIntro; done.
+        - iDestruct (big_sepM_delete with "Haddrs_match") as
+              "[_ ?]"; [eauto | done].
+      }
+      iPureIntro.
+      split.
+      * eapply sent_consistent_after_send;
+          [assumption | eapply Hsome | set_solver ].
+      * eapply recv_consistent_after_send;
+          [assumption | apply Hsome | by rewrite Heq].
+  Qed.
+End client.
+
+Section server.
+  Context `{!NetworkTopo}.
+  Context `{!GhostInvNames}.
+  Context `{!inG Σ freeUR}.
+  Context `{!inG Σ handlesUR}.
+  Context `{!inG Σ pingTokR}.
+  Context `{distG : !anerisG ping_pong_model Σ}.
+
+  Definition server_si : socket_interp Σ :=
+    (λ msg, ∃ a, ⌜a ∈ n_clients /\ msg = mkPing a⌝)%I.
+
+  Definition set_match_list (addrs : gset socket_address) (addrs': list socket_address): Prop :=
+    list_to_set addrs' = addrs.
+
+  Fixpoint client_addrs (addrs : list socket_address) : base_lang.expr :=
+    match addrs with
+    | nil => list_nil
+    | a :: addrs' => list_cons #a (client_addrs addrs')
+    end.
+
+  Lemma server_spec (ip : ip_address) l l':
+    (set_match_list n_clients l') ->
+    (is_list (map (LitV ∘ LitSocketAddress) l') l) ->
+    ip = ip_of_address n_server ->
+    {{{ inv inv_ns ping_pong_inv ∗
+        fixed n_all ∗
+        ufree n_server ∗
+        n_server ⤇ server_si }}}
+      server #n_server l  @[ip]
+    {{{ v, RET v; True }}}.
+  Proof. Admitted.
+
+End server.
+
+Section topo.
+
+  Definition mkAddr ip := SocketAddressInet ip 80.
+  Global Instance ping_pong_topo : NetworkTopo.
+  Proof.
+    apply (mkTopo (mkAddr "0.0.0.99")
+                  {[ mkAddr "0.0.0.1"; mkAddr "0.0.0.2"; mkAddr "0.0.0.3" ]}).
+    set_solver.
+  Defined.
+End topo.
+
+Section alloc.
+
+  Context `{NetworkTopo}.
+  Context `{inG Σ freeUR}.
+  Context `{!inG Σ handlesUR}.
+  Context `{!inG Σ pingTokR}.
+
+  From iris Require Import algebra.auth.
+
+  Definition ping_tok' (f: gmap socket_address gname) (a : socket_address) : iProp Σ :=
+    match (f !! a) with
+    | Some γ => own γ (Excl 0)
+    | None => True
+    end.
+
+  Lemma alloc_tokens (addrs: gset socket_address):
+    ⊢ |==> ∃ f, ⌜ dom (gset _) f = addrs ⌝ ∧ [∗ set] addr ∈ addrs, ping_tok' f addr.
+  Proof.
+    induction addrs as [|x X Hnotin IH] using set_ind_L.
+    { iModIntro. iExists ∅. iSplit=>//. iPureIntro; set_solver. }
+    iStartProof.
+    iMod (own_alloc (Excl 0)) as (γ) "Hγ" =>//.
+    iMod IH as (f) "[%Hdom H]".
+    iExists (<[x:=γ]>f).
+    iModIntro; iSplit.
+    { iPureIntro. set_solver. }
+    iApply big_sepS_insert=>//; iSplitL "Hγ".
+    - by rewrite /ping_tok' lookup_insert.
+    - iApply (big_sepS_impl with "H").
+      iIntros "!>" (y Hy) "H".
+      rewrite /ping_tok' lookup_insert_ne =>//.
+      by set_solver.
+  Qed.
+
+  Lemma toto `{!inG Σ (X:ucmra)} γ (A B: X):
+    A ≡ B ->
+    own γ A ⊣⊢ own γ B.
+  Proof. by move=> ->. Qed.
+
+  Lemma union_singletons A `{GhostInvNames}:
+    own γ_free (◯ GSet A) ⊢
+        own proof.γ_free (◯ ([^op set] x ∈ A, GSet {[x]})).
+  Proof.
+    iIntros "H".
+    rewrite toto => //.
+    f_equiv.
+    induction A as [|x X Hnotin IH] using set_ind_L.
+    { by rewrite big_opS_empty. }
+    rewrite big_opS_insert //. rewrite -IH -gset_disj_union //; last set_solver.
+  Qed.
+
+  Lemma alloc_gnames: (⊢ |==> ∃c: GhostInvNames,
+                            ([∗ set] a ∈ n_all, ufree a) ∗
+                            own γ_free (● GSet n_all) ∗
+                            auth_handles ∅ ∗ own γ_handles (◯ (handles_to_excl ∅)) ∗
+                            ([∗ set] a ∈ n_clients, ping_tok a)
+                      ).
+  Proof.
+    iMod (own_alloc (● GSet n_all ⋅ ◯ GSet n_all)) as (γ_free) "[Hfree Hfree']".
+    { apply auth_both_valid_2; eauto. by compute. }
+    iMod (alloc_tokens n_clients) as (f_tokens) "[%Htokdom Htoks]".
+    iMod (own_alloc (● handles_to_excl ∅ ⋅ ◯ handles_to_excl ∅)) as (γ_handles) "Hh".
+    { apply auth_both_valid_2; eauto. vm_compute. done. }
+
+    iModIntro.
+    iExists {| gen_tok_name := fun a => f_tokens !! a ;
+               γ_free := γ_free ;
+               γ_handles := γ_handles ;
+               inv_ns := nroot .@ "iterated_ping_pong"
+            |}.
+    iFrame. rewrite !own_op. iFrame.
+    rewrite /ufree -big_opS_own; last set_solver.
+    rewrite -big_opS_commute1; last set_solver.
+    by rewrite -union_singletons.
+
+    Unshelve.
+    - intros a Hin. apply elem_of_dom. congruence.
+  Qed.
+
+  Definition protomap `{GhostInvNames} `{anerisG ping_pong_model Σ}: socket_address -> socket_interp Σ :=
+    fun a => if decide (a = mkAddr "0.0.0.99") then server_si else client_si a.
+
+End alloc.
+
+Section runner.
+
+  Definition invN := nroot .@ "ping_pong".
+
+  Context `{!inG Σ freeUR}.
+  Context `{!inG Σ handlesUR}.
+  Context `{!inG Σ pingTokR}.
+  Context `{!GhostInvNames}.
+  Context `{distG : !anerisG ping_pong_model Σ}.
+
+
+  Lemma runner_spec :
+    {{{ n_server ⤇ server_si
+        ∗ ([∗ set] a ∈ n_clients, a ⤇ client_si a)
+        ∗ fixed n_all
+        ∗ ([∗ set] a ∈ n_all, free_ip (ip_of_address a))
+        ∗ ([∗ set] a ∈ n_all, a ⤳ (∅, ∅))
+        ∗ ([∗ set] a ∈ n_all, ufree a)
+        ∗ inv inv_ns ping_pong_inv
+    }}}
+      runner @["system"]
+    {{{ v, RET v; True }}}.
+  Proof.
+    iIntros (Φ) "(Hserver & Hprotos & #Hfixed & Hips & Hlts & Hufrees & #Hinv) Hkont". rewrite /runner.
+    rewrite /n_clients /ping_pong_topo.
+    iDestruct (big_sepS_delete _ _ (mkAddr "0.0.0.1") with "Hips") as "[Hn1 Hips]"; first set_solver.
+    iDestruct (big_sepS_delete _ _ (mkAddr "0.0.0.2") with "Hips") as "[Hn2 Hips]"; first set_solver.
+    iDestruct (big_sepS_delete _ _ (mkAddr "0.0.0.3") with "Hips") as "[Hn3 Hips]"; first set_solver.
+    iDestruct (big_sepS_delete _ _ (mkAddr "0.0.0.99") with "Hips") as "[Hns _]"; first set_solver.
+
+    iDestruct (big_sepS_delete _ _ (mkAddr "0.0.0.1") with "Hlts") as "[Hlt1 Hlts]"; first set_solver.
+    iDestruct (big_sepS_delete _ _ (mkAddr "0.0.0.2") with "Hlts") as "[Hlt2 Hlts]"; first set_solver.
+    iDestruct (big_sepS_delete _ _ (mkAddr "0.0.0.3") with "Hlts") as "[Hlt3 Hlts]"; first set_solver.
+    iDestruct (big_sepS_delete _ _ (mkAddr "0.0.0.99") with "Hlts") as "[Hlts _]"; first set_solver.
+
+    iDestruct (big_sepS_delete _ _ (mkAddr "0.0.0.1") with "Hprotos") as "[Hp1 Hprotos]"; first set_solver.
+    iDestruct (big_sepS_delete _ _ (mkAddr "0.0.0.2") with "Hprotos") as "[Hp2 Hprotos]"; first set_solver.
+    iDestruct (big_sepS_delete _ _ (mkAddr "0.0.0.3") with "Hprotos") as "[Hp3 _]"; first set_solver.
+
+    iDestruct (big_sepS_delete _ _ (mkAddr "0.0.0.1") with "Hufrees") as "[Hu1 Hufrees]"; first set_solver.
+    iDestruct (big_sepS_delete _ _ (mkAddr "0.0.0.2") with "Hufrees") as "[Hu2 Hufrees]"; first set_solver.
+    iDestruct (big_sepS_delete _ _ (mkAddr "0.0.0.3") with "Hufrees") as "[Hu3 Hufrees]"; first set_solver.
+    iDestruct (big_sepS_delete _ _ (mkAddr "0.0.0.99") with "Hufrees") as "[Hus _]"; first set_solver.
+
+    do 3 (wp_makeaddress; wp_let). (* Lots of time in typeclasses eauto 🐌 *)
+
+    wp_bind (list_nil).
+    wp_apply wp_list_nil. done. iIntros (vv1 Hvv1).
+    wp_bind (list_cons _ vv1).
+    wp_apply wp_list_cons. done. iIntros (vv2 Hvv2).
+    wp_bind (list_cons _ vv2).
+    wp_apply wp_list_cons. done. iIntros (vv3 Hvv3).
+    wp_bind (list_cons _ vv3).
+    wp_apply wp_list_cons. done. iIntros (vv4 Hvv4).
+
+    clear Hvv1 vv1 Hvv2 vv2 Hvv3 vv3.
+    pose proof Hvv4 as HH.
+    do 3 destruct Hvv4 as [? [-> Hvv4]]. rewrite Hvv4. rewrite Hvv4 in HH.
+
+    wp_pures.
+
+    wp_bind (Start _ _).
+    wp_apply (aneris_wp_start {[80%positive]} with "[-]"); eauto. iFrame.
+    iSplitR "Hp1 Hu1 Hlt1"; first last.
+    { iModIntro. iIntros "Hfp".
+      wp_apply (client_spec with "[$] [] [$] [$] [$] [-]"); eauto.
+      set_solver. }
+    iModIntro. wp_pures.
+    wp_apply (aneris_wp_start {[80%positive]} with "[-]"); auto. iFrame.
+    iSplitR "Hp2 Hu2 Hlt2"; first last.
+    { iModIntro. iIntros "Hfp".
+      wp_apply (client_spec with "[$] [] [$] [$] [$] [-]"); eauto.
+      set_solver. }
+    iModIntro. wp_pures.
+    wp_apply (aneris_wp_start {[80%positive]} with "[-]"); auto. iFrame.
+    iSplitR "Hp3 Hu3 Hlt3"; first last.
+    { iModIntro. iIntros "Hfp".
+      wp_apply (client_spec with "[$] [] [$] [$] [$] [-]"); eauto.
+      set_solver. }
+
+    iModIntro. wp_pures.
+    wp_apply (aneris_wp_start {[80%positive]} with "[-]"); auto. iFrame.
+
+    iSplitL "Hkont"; first by iApply "Hkont".
+    iModIntro. iIntros "_".
+    iApply (server_spec _ _ [mkAddr "0.0.0.1"; mkAddr "0.0.0.2"; mkAddr "0.0.0.3"] with "[-]"); eauto.
+    { set_solver. }
+  Qed.
+
+End runner.
+
+Lemma big_sepS_map_inverse `{Σ: gFunctors} `{Countable A} `{Countable B} (X: gset A)
+        (f: A -> B) (g: B -> A) (P: A -> iProp Σ):
+    (forall x, g (f x) = x) ->
+    (([∗ set] x ∈ set_map f X, P (g x)) ⊣⊢ [∗ set] x ∈ X, P x)%I.
+Proof.
+  intros Hinv. induction X as [| x X Hnotin IH] using set_ind_L.
+  { iStartProof. iSplit; iIntros "?"; done. }
+  iStartProof.
+  rewrite set_map_union_L.
+  rewrite big_sepS_union; try set_solver; last first.
+  - have Hfinj: forall x y, f x = f y -> x = y.
+    { move=> a b Hab. have: g (f a) = g (f b) by f_equal. congruence. }
+    move=> a Hs Hr.
+    rewrite -> elem_of_map in Hs. destruct Hs as (x' & Heq & Hs).
+    rewrite -> elem_of_map in Hr. destruct Hr as (y & Heq' & Hr).
+    subst. apply Hfinj in Heq'. set_solver.
+  - rewrite big_sepS_union; last set_solver.
+    rewrite set_map_singleton_L !big_sepS_singleton. rewrite Hinv.
+    iSplit; iIntros "[??]"; iFrame; by iApply IH.
+Qed.
+
+
+Lemma big_sepS_duh `{Σ: gFunctors} `{Countable A} `{Countable B} (X Y: gset A)
+         (P: A -> iProp Σ):
+  X = Y ->
+    (([∗ set] x ∈ X, P x) ⊣⊢ [∗ set] x ∈ Y, P x)%I.
+Proof.
+  iIntros (Heq). rewrite Heq. reflexivity.
+Qed.
+
+Section simulation.
+  (* Bug in coq! please report to coq.inria.fr *)
+  (* Definition mkAddrPair (a: ip_address): ip_address * (gset _) := (a, {[ 80 ]}). *)
+
+  (* Definition mkAddrPair (a: ip_address): ip_address * (gset port) := (a, {[ 80%positive ]}). *)
+  Definition mkAddrPair (a: ip_address): ip_address * (gset port) := (a, ∅).
+
+  Definition n_all_piu: ports_in_use :=
+    list_to_map [ mkAddrPair "0.0.0.1"; mkAddrPair "0.0.0.2"; mkAddrPair "0.0.0.3"; mkAddrPair "0.0.0.99" ].
+
+  Definition initial_state: state aneris_lang := {|
+    state_heaps := {["system" := ∅]};
+    state_sockets := {["system" := ∅]};
+    state_ports_in_use := n_all_piu;
+    state_ms := ∅ |}.
+
+  (* Notice we're using the previously-declared NetworkTopo.
+     This is required as an implicit argument of ping_pong_model. *)
+
+  Definition simulates (ex : execution_trace aneris_lang)
+                       (sm : auxiliary_trace (@aneris_AS ping_pong_model)) : Prop :=
+    exists (conf : cfg aneris_lang) (curr_st : ping_pong_model) (mh: messages_history) curr_δ,
+      exec_ends_in ex conf /\
+      auxtr_ends_in sm curr_δ /\
+      curr_st = curr_δ.(aneris_AS_model) ∧
+      mh = curr_δ.(aneris_AS_mhist) ∧
+      match (snd conf) with
+        mkState _ c_skts c_in_use _ =>
+        exists (P F : gset socket_address) (handles : handle_map),
+        P ## F /\
+        (* The tracked addresses match physical addresses on the network *)
+        (* P ∪ F = n_all /\ *)
+        (* The participating addresses are the keys in the handle map *)
+        dom _ handles = P /\
+        (* The participating sockets are allocated *)
+        (* ([^ and map] a ↦ hst ∈ handles, hst.(skt).(saddress) = Some a) /\ *)
+        (* (* Free addresses really are free *) *)
+        (* ([^ and set] a ∈ F, *)
+        (*   match c_in_use !! (ip_of_address a) with *)
+        (*     None => True *)
+        (*   | Some ports => port_of_address a ∉ ports *)
+        (*   end) /\ *)
+        (* Our tracking of sends is consistent with the model *)
+        sent_consistent curr_st handles /\
+        (* Our tracking of receives is consistent with the model *)
+        recv_consistent curr_st handles /\
+        forall a, a ∈ P -> ∃ hst, handles !! a = Some hst ∧
+              (forall m, m ∈ hst.(sent) -> (m.(m_sender) = a ∧ m ∈ mh.2))
+      end.
+
+  Definition runner_expr: expr aneris_lang := mkExpr "system" runner.
+
+
+  From stdpp Require Import sets.
+  From aneris Require Import lib.util.
+
+  (* Lemma big_sepS_gset_map Φ Ψ X f g: *)
+  (*  forall x, f (g x) = x *)
+  (*   ([∗ set] x ∈ X, Φ x) -∗ *)
+  (*   [∗ set] x ∈ (gset_map f X), Ψ (g x). *)
+
+  Class ppG Σ := { free_ur_inG:> inG Σ freeUR
+                 ; handles_inG:> inG Σ handlesUR
+                 ; pingtok_inG:> inG Σ pingTokR }.
+
+  Definition myΣ: gFunctors := #[ anerisΣ ping_pong_model
+                                ; GFunctor freeUR
+                                ; GFunctor handlesUR
+                                ; GFunctor pingTokR ].
+
+  Instance subG_ppΣ {Σ}: subG myΣ Σ -> ppG Σ.
+  Proof. solve_inG. Qed.
+
+  (* Instance whatamidoing: anerisG myΣ ping_pong_model. *)
+  (* Proof. Admitted. *)
+
+  From stdpp Require Import fin_sets.
+  From aneris.aneris_lang Require Import adequacy.
+
+  Theorem ping_pong_simulation :
+    continued_simulation
+      simulates
+      (singleton_exec (([runner_expr], initial_state)))
+      (@singleton_auxtr _ (@aneris_AS ping_pong_model)
+         {| aneris_AS_mhist := (∅,∅) ; aneris_AS_model := []:ping_pong_model |}).
+  Proof.
+    eapply (simulation_adequacy
+              myΣ _
+              NotStuck
+              {[ "0.0.0.1"; "0.0.0.2"; "0.0.0.3"; "0.0.0.99" ]}
+              n_all);
+      eauto; try set_solver.
+    { admit. (* finite branching *) }
+    { move => a Ha. unfold n_all, n_clients in Ha. set_solver. }
+    move=> Haneris. iStartProof.
+    iMod alloc_gnames as (?) "(Hufrees&Hfreeall&Hah&Hfh&Htok)".
+    iModIntro.
+    iExists (λ v, ∃ w, ⌜v = mkVal "system" w⌝ ∗ (fun _ => True) w)%I, protomap.
+    iIntros "#Hfixed Hprotos Hlts Hfrees Hsystemnode Hfragst".
+
+    iMod (inv_alloc inv_ns _ ping_pong_inv with "[-Hlts Hufrees Hsystemnode Hprotos Hfrees]") as "#Hinv".
+    { iNext. rewrite /ping_pong_inv. iExists ∅. iSplitR "Htok".
+      - rewrite /generic_inv. iExists ∅, n_all, ∅. iFrame.
+        iSplit. iPureIntro; set_solver.
+        iSplit. iPureIntro; set_solver.
+        iSplitL "". { unfold handle_addrs_match. done. }
+        iSplitL "". { unfold mapsto_handles. eauto. }
+        iSplit; eauto.
+      - iApply (big_sepS_impl with "Htok") =>//.
+          by iIntros "!>" (a Ha) "Hpk"; iLeft.
+    }
+    iSplitL.
+    - iApply fupd_wp.
+
+      iRevert "Hsystemnode".
+      iAssert (aneris_wp_def "system" ⊤ runner ⊤)%I with "[-]" as "H"; first last.
+      { rewrite /aneris_wp_def. iIntros "Hnode". iSpecialize ("H" with "Hnode").
+        iExact "H". }
+      rewrite -aneris_wp_eq.
+      iAssert (WP runner @["system"] {{⊤}})%I with "[-]" as "H"; last by eauto.
+      wp_apply (runner_spec with "[-]"); eauto.
+
+      iDestruct (big_sepS_delete _ _ (mkAddr "0.0.0.99") with "Hprotos") as "[Hserverproto Hprotos]"; first set_solver.
+      rewrite {1}/protomap /=.
+      destruct (decide (mkAddr "0.0.0.99" = mkAddr "0.0.0.99")); [|done].
+      iFrame "# Hserverproto". iSplitL "Hprotos".
+      { have ->: {[mkAddr "0.0.0.1"; mkAddr "0.0.0.2"; mkAddr "0.0.0.3"]} =
+          (n_all ∖ {[mkAddr "0.0.0.99"]}) by rewrite /n_all; set_solver.
+        iApply (big_sepS_impl with "Hprotos").
+        iModIntro. iIntros (x Hx) "H".
+        rewrite /protomap. destruct (decide (x = mkAddr "0.0.0.99")) as [->|];
+                             first by set_solver. done. }
+      iFrame.
+      iPoseProof (big_sepS_map_inverse _ mkAddr ip_of_address with "Hfrees") as "H"=> //.
+      assert (Heq: n_all = set_map mkAddr (C := gset _) {["0.0.0.1"; "0.0.0.2"; "0.0.0.3"; "0.0.0.99"]}).
+      { unfold mkAddr, n_all, n_clients, ping_pong_topo, n_server. set_solver. }
+      rewrite Heq. iExact "H".
+    - do 2 iModIntro.
+      iIntros (ex atr δ' c' κs' Hval Hexst Hauxst Hexend Hauxend).
+      iIntros (Hsim Hnotstuck) "Hsi Hposts".
+      iInv inv_ns as "> Hgi" "Hclose".
+
+      unfold simulates.
+      unfold ping_pong_inv.
+      iDestruct "Hgi" as (mdl) "[Hgi ?]".
+      iDestruct "Hgi" as (P F handles) "(%&?&%&?&Hhandles&Hm&Hfrag&%&%)".
+
+      unfold handle_addrs_match, handle_addr_match,
+        mapsto_handles, handle_st_to_mapsto.
+      iAssert (⌜ ∀ a : socket_address,
+                    a ∈ dom (gset socket_address) handles
+                    → ∃ hst : HandleSt,
+                      handles !! a = Some hst
+                      ∧ (∀ m : message, m ∈ sent hst ->
+                      m_sender m = a ∧ m ∈ (aneris_AS_mhist δ').2) ⌝)%I as "%".
+      { iIntros (a Ha). apply elem_of_dom in Ha as [hst Ha]. iExists hst.
+        iSplit; first done. iIntros (m Hm).
+
+        iDestruct (big_sepM_delete _ handles _ hst Ha with "Hhandles")
+          as "[[? [? H]] _]".
+        iDestruct (big_sepM_delete _ handles _ hst Ha with "Hm")
+          as "[[_ Hahist] _]".
+        iSplit; first by
+            iDestruct (big_sepS_delete _ (sent hst) m Hm with "H") as "[? _]".
+        iDestruct (aneris_state_interp_sent_mapsto_agree with "Hahist Hsi")
+          as "%Hx". rewrite <- Hx in *.
+        iPureIntro.
+
+        unfold messages_sent_from in Hx. destruct δ'. simpl in *.
+        set_solver.
+      }
+
+      unfold mapsto_handles, handle_st_to_mapsto.
+
+      iAssert (⌜δ'.(aneris_AS_model)  = mdl ⌝)%I with "[Hsi Hfrag]" as "%".
+      { iApply (aneris_state_interp_model_agree with "Hsi Hfrag").  }
+      subst.
+
+      iApply (fupd_mask_weaken ∅); first set_solver. iIntros "_ !>".
+
+      (* iPoseProof (socket_state_same with "[$] [$]") as "%Hsame". *)
+      iPureIntro. eexists c', δ'.(aneris_AS_model), δ'.(aneris_AS_mhist), δ'.
+      split. eauto using exec_extend_ends_in.
+      split. eauto using auxtr_extend_ends_in.
+      split. done.
+      split. done.
+      destruct c'.2.
+      eexists _, F, handles.
+      do 4 (split; eauto).
+  Admitted.
+
+End simulation.
